ifc-machine/pico/tmu/cmach/Refinement.v
@@ -7,7 +7,7 @@ Require Import Utils Lattices CLattices.
 Require Import TMUInstr.
 Require Import Abstract Rules AbstractMachine.
 
-Require Import Concrete ConcreteMachine CodeGen.
+Require Import Concrete ConcreteMachine CodeGen CodeSpecs.
 Require Import FaultRoutine.
 
 Require Import Simulation.
@@ -24,8 +24,6 @@ Context {L: Type}
 
 (** The fault handler code *)
 Definition faultHandler := CodeGen.faultHandler fetch_rule.
-Definition valid_cache {T: Type} (l: list T) := eq tmuCacheSize (length l).
-Definition valid_fh {T: Type} (l : list T) := eq privInstSize (length l).
 
 Inductive match_stacks : list (@StkElmt L) ->  list (@CStkElmt L) -> Prop :=
 | ms_nil : match_stacks nil nil
@@ -38,27 +36,13 @@ Inductive match_stacks : list (@StkElmt L) ->  list (@CStkElmt L) -> Prop :=
 
 Inductive match_states : @AS L -> @CS L -> Prop :=
 |  ms: forall m i astk cstk pc tmuc fh
-              (STKS: match_stacks astk cstk)
-              (CACHE: valid_cache tmuc) 
-              (FH: valid_fh fh),
+              (STKS: match_stacks astk cstk),
          match_states (AState m i astk pc)
-                      (CState (tmuc++m) (fh++i) cstk pc false)
+                      (CState tmuc m fh i cstk pc false)
 .
 
-Check forward_backward_sim.
-
 (** Aux functions yet to be defined - or specified at least *)
-Variable drop_cache : list (@Atom L) -> list (@Atom L).
-Variable drop_fhandler : list (@Instr L) -> list (@Instr L).
 Variable c_to_a_stack : list (@CStkElmt L) -> list (@StkElmt L). 
-
-Axiom drop_cache_correct: forall c m, 
-    valid_cache c ->
-    drop_cache (c++m) = m.
-
-Axiom drop_fhandler_correct: forall h i, 
-    valid_fh h ->
-    drop_fhandler (h++i) = i.
 
 Axiom match_stacks_obs : forall s s', 
     match_stacks s s' ->
@@ -67,7 +51,7 @@ Axiom match_stacks_obs : forall s s',
 (** Observing a concete cache is just projecting it a the abstract level *)
 Definition observe_cstate (cs: @CS L) : @AS L := 
   match cs with 
-    | CState m i s pc p => AState (drop_cache m) (drop_fhandler i) (c_to_a_stack s) pc
+    | CState c m fh i s pc p => AState m i (c_to_a_stack s) pc
   end.
 
 (* DD: Don't be tempted to add success s1 as a hyothesis... *)
@@ -77,7 +61,7 @@ Axiom final_step_preserved:
     (match_states s1 s2) ->
     (forall s2', ~ cstep s2 s2')
     /\ s1 = observe_cstate s2.
-
+     
 Axiom step_preserved: 
   forall s1 s1' s2,
     step_rules s1 s1' ->
@@ -89,12 +73,247 @@ Axiom succ_preserved:
     match_states s1 s2 -> 
     success s1 <-> c_success s2.
 
-Axiom cmach_determ: 
+Ltac allinv' :=
+  allinv ; 
+    (match goal with 
+       | [ H1:  ?f _ _ = _ , 
+           H2:  ?f _ _ = _ |- _ ] => rewrite H1 in H2 ; inv H2
+     end).
+  
+
+Lemma app_same_length_eq (T: Type): forall (l1 l2 l3 l4: list T), 
+  l1++l2 = l3++l4 -> 
+  length l1 = length l3 ->
+  l1 = l3.
+Proof.
+  induction l1; intros; simpl in *.
+  destruct l3; auto. inv H0.
+  destruct l3. inv H0. simpl in *.
+  inv H. erewrite IHl1 ; eauto.
+Qed.  
+
+Lemma app_same_length_eq_rest (T: Type): forall (l1 l2 l3 l4: list T), 
+  l1++l2 = l3++l4 -> 
+  length l1 = length l3 ->
+  l2 = l4.
+Proof.
+  intros.
+  exploit app_same_length_eq; eauto.
+  intro Heq ; inv Heq.
+  gdep l3. induction l3 ; intros; auto.
+  simpl in *.
+  inv H. eauto.
+Qed.
+  
+Lemma cmach_priv_determ: 
+  forall s s' s'', 
+    cstep_p s s' -> 
+    cstep_p s s'' -> 
+    s' = s''.
+Proof.
+  induction 1; intros; 
+  match goal with 
+      | [HH: cstep_p _ _ |- _ ] => inv HH; try congruence; auto
+  end;
+  (allinv'; try reflexivity).
+  
+  Case "Call".
+    exploit app_same_length_eq; eauto. intro Heq ; inv Heq.
+    exploit app_same_length_eq_rest ; eauto. intro Heq ; inv Heq.
+    reflexivity.
+
+  Case "Ret".
+    exploit @c_pop_to_return_spec; eauto.
+    intros [dstk [stk [a [b [p [Hs Hdstk]]]]]]. inv Hs.
+    
+    exploit @c_pop_to_return_spec2; eauto.  move_to_top H11.
+    exploit @c_pop_to_return_spec2; eauto. intros. 
+    inv H1. inv H2. 
+    
+    exploit @c_pop_to_return_spec3; eauto. clear H0.
+    exploit @c_pop_to_return_spec3; eauto. intros.
+    inv H1. 
+    reflexivity.
+    
+  Case "VRet".
+    exploit @c_pop_to_return_spec; eauto.
+    intros [dstk [stk [a [b [p [Hs Hdstk]]]]]]. inv Hs.
+
+    exploit @c_pop_to_return_spec2; eauto. intros. move_to_top H13.
+    exploit @c_pop_to_return_spec2; eauto. intros. 
+
+    exploit @c_pop_to_return_spec3; eauto. intros. 
+    generalize H13 ; clear H13 ; intros H13.
+    exploit @c_pop_to_return_spec3; eauto. intros.
+    inv H1. inv H2.
+    reflexivity.
+Qed.
+
+Lemma cache_hit_same_content (T: Type): forall opcode op1 op2 op3 pcl c c',
+  cache_hit c (mvector opcode op1 op2 op3 pcl) ->
+  cache_hit c' (mvector opcode op1 op2 op3 pcl) ->
+  forall a, 
+    (a = addrOpLabel \/ a = addrTag1 \/ a = addrTag2 \/ a = addrTag3 \/ a = addrTagPC) ->
+    index_list_Z a c = index_list_Z a c'.
+Proof.
+  intros. inv H; inv H0. 
+  intuition; match goal with | [HH: a = _ |- _ ] => inv HH end.
+  inv OP0. inv OP. congruence.
+  destruct op1; inv TAG1 ; inv TAG0; congruence.
+  destruct op2; inv TAG2 ; inv TAG4; congruence.
+  destruct op3; inv TAG3 ; inv TAG5; congruence.
+  inv TAGPC ; inv TAGPC0; congruence.
+Qed.  
+
+Lemma index_list_cons (T: Type): forall n a (l:list T),
+ index_list n l = index_list (n+1) (a :: l).
+Proof.
+  intros.
+  replace ((n+1)%nat) with (S n) by omega. 
+  gdep n. induction n; intros.
+  destruct l ; simpl; auto.
+  destruct l. auto. 
+  simpl. eauto.
+Qed. 
+
+Lemma index_list_Z_cons (T: Type): forall i (l1: list T) a, 
+  i >= 0 ->
+  index_list_Z i l1 = index_list_Z (i+1) (a::l1).
+Proof.
+  induction i; intros.
+  auto.
+  simpl. unfold read_m. simpl. 
+  replace (Pos.to_nat (p + 1)) with ((Pos.to_nat p)+1)%nat by (zify; omega).
+  eapply index_list_cons ; eauto. 
+  zify; omega.
+Qed. 
+  
+Lemma index_list_Z_eq (T: Type) : forall (l1 l2: list T), 
+  (forall i, index_list_Z i l1 = index_list_Z i l2) ->
+  l1 = l2.
+Proof.
+  induction l1; intros.
+  destruct l2 ; auto.
+  assert (HCont:= H 0). unfold read_m in HCont. inv HCont. 
+  destruct l2.
+  assert (HCont:= H 0). unfold read_m in HCont. inv HCont. 
+  assert (a = t). 
+  assert (Helper:= H 0). unfold read_m in Helper. inv Helper. auto.
+  inv H0. 
+  erewrite IHl1 ; eauto.
+  intros. destruct i.
+  erewrite index_list_Z_cons with (a:= t); eauto; try omega.
+  erewrite H ; eauto.  
+  erewrite index_list_Z_cons with (a:= t); eauto; try (zify ; omega).
+  erewrite H ; eauto. symmetry. eapply index_list_Z_cons; eauto. zify; omega.
+  destruct l1, l2 ; auto.
+Qed.
+  
+Lemma check_cache_determ: forall opcode op1 op2 op3 pcl cs cs' cs'',
+  check_tags opcode op1 op2 op3 pcl cs cs' ->
+  check_tags opcode op1 op2 op3 pcl cs cs'' ->
+  cs' = cs''.
+Proof.
+  induction 1 ; intros; inv H; auto; try (solve [ intuition]).
+  unfold update_cache_spec_mvec in *.
+  assert (H_OTHERS: forall addr,  addr <> addrOpLabel ->  addr <> addrTagPC -> 
+                        addr <> addrTag1 -> addr <> addrTag2 -> addr <> addrTag3 ->
+                        read_m addr c' = read_m addr c'0) by
+      (intros; rewrite <- UPD; auto).
+  generalize (cache_hit_same_content L C'HIT C'HIT0). intros Hid.
+  cut (c' = c'0). intros Heq ; inv Heq. auto.
+
+  eapply index_list_Z_eq ; eauto.
+  intros. 
+  destruct (Z_eq_dec i0 addrOpLabel).
+    inv e. eauto. destruct (Z_eq_dec i0 addrTag1).
+    inv e. eauto. destruct (Z_eq_dec i0 addrTag2).
+    inv e. eauto. destruct (Z_eq_dec i0 addrTag3).
+    inv e. eapply Hid; eauto. destruct (Z_eq_dec i0 addrTagPC).
+    inv e. eapply Hid; eauto. eapply H_OTHERS; eauto.
+Qed.
+
+Lemma runsToEnd'_pc_increase {T: Type}: forall (step: @CS T -> @CS T -> Prop) n n' cs cs',
+  runsToEnd' step n n' cs cs'  -> 
+  n <= n' .
+Proof.
+  induction 1; intros.
+  omega.
+  omega.
+Qed.
+
+Lemma runsToEnd'_determ {T: Type}: forall (step: @CS T -> @CS T -> Prop)
+                                  (step_determ: forall s1 s2 s2', step s1 s2 -> step s1 s2' -> s2 = s2')
+                                  n n' cs cs',
+   runsToEnd' step n n' cs cs' ->
+   forall  cs'', runsToEnd' step n n' cs cs'' ->
+   cs' = cs''.
+Proof.
+  induction 2; intros.
+  
+  inv H0. auto.
+          eapply @runsToEnd'_pc_increase in H5; eauto. zify ; omega.
+
+  inv H3; inv H4.
+  zify ; omega.
+  
+  assert (Heq: cs' = cs''). eapply step_determ; eauto. inv Heq.
+  eapply IHrunsToEnd' ; eauto.  
+
+  eapply @runsToEnd'_pc_increase in H9; eauto. zify ; omega.
+  
+  assert (Heq: cs' = cs'1). eapply step_determ; eauto. inv Heq.
+  eapply IHrunsToEnd' ; eauto.  
+Qed.
+  
+Lemma runsToEscape_determ {T: Type}: forall (step: @CS T -> @CS T -> Prop)
+                                  (step_determ: forall s1 s2 s2', step s1 s2 -> step s1 s2' -> s2 = s2')
+                                  n n' cs cs' cs'',
+   runsToEscape step n n' cs cs' ->
+   runsToEscape step n n' cs cs'' ->
+   cs' = cs''.
+Proof.
+  induction 2 ; intros.
+  { inv H. 
+    - assert (Heq: cs'0 = cs') by (eapply runsToEnd'_determ; eauto). inv Heq.
+    eapply step_determ; eauto.
+  
+    - assert (Heq: cs' = cs'') by (eapply runsToEnd'_determ; eauto). inv Heq.
+      eelim FAIL ; eauto. 
+  }
+  { inv H.
+    - assert (Heq: cs'0 = cs') by (eapply runsToEnd'_determ; eauto). inv Heq.
+      eelim FAIL ; eauto.
+      
+    - eapply runsToEnd'_determ; eauto.
+  }
+Qed.  
+   
+Lemma run_tmu_determ: forall opcode op1 op2 op3 pcl cs cs' cs'',
+  run_tmu opcode op1 op2 op3 pcl cs cs' ->
+  run_tmu opcode op1 op2 op3 pcl cs cs'' ->
+  cs' = cs''.
+Proof.
+  induction 1; intros; inv H3.
+  replace cs'0 with cs' in * by (eapply check_cache_determ ; eauto).
+  eapply runsToEscape_determ; eauto.
+  eapply cmach_priv_determ; eauto.
+Qed.
+
+Lemma cmach_determ: 
   forall s s' s'', 
     cstep s s' -> 
     cstep s s'' -> 
     s' = s''.
- 
+Proof.
+  induction 1 ; intros;
+  match goal with 
+    | [HH: cstep _ _ |- _ ] => inv HH; try congruence; auto
+  end;
+    (allinv'; try reflexivity).
+Admitted.
+
+
 Require Import LNIwithEvents.
 
 Let aexec_with_trace := sys_trace step_rules success (fun x => x).
